all functions on finite domains are continous

LeanScratch/Domain/Finite.lean
@@ -5,6 +5,7 @@ import LeanScratch.Domain.Dom
 import LeanScratch.Domain.Lub
 import LeanScratch.Domain.Continous
 import LeanScratch.Fin2
+import LeanScratch.HEq
 
 namespace Dom
 
@@ -27,8 +28,8 @@ structure Finite (c : C α) : Type _ where
   ls : List α
   ordered : List.Pairwise ida.lt ls
 
-  extractor (n : Nat) : Fin2 ls.length
-  extractor_agrees (n : Nat) : c n = ls.getFin2 (extractor n)
+  extractor (n : Nat) : Fin ls.length
+  extractor_agrees (n : Nat) : c n = ls.get (extractor n)
   sur : Function.Surjective extractor
 
 namespace Finite
@@ -39,15 +40,15 @@ noncomputable def extractor.of
     {ls : List α}
     (allMem : ∀ n, c n ∈ ls)
     (n : Nat)
-    : Fin2 ls.length :=
-  Classical.choose $ Fin2.ofMem $ allMem n
+    : Fin ls.length :=
+  Classical.choose $ List.mem_iff_get.mp $ allMem n
 
 theorem extractor_agrees.of
     {ls : List α}
     {allMem : ∀ n, c n ∈ ls}
     (n : Nat)
-    : c n = ls.getFin2 (extractor.of allMem n) :=
-  Classical.choose_spec (p := λ x ↦ c n = ls.getFin2 x) $ Fin2.ofMem $ allMem n
+    : c n = ls.get (extractor.of allMem n) :=
+  (Classical.choose_spec $ List.mem_iff_get.mp $ allMem n).symm
 
 def nodup (f : Finite c) : f.ls.Nodup :=
   f.ordered.rec .nil
@@ -59,8 +60,8 @@ theorem sur.of
     (nodup : ls.Nodup)
     (memAll : (x : α) → x ∈ ls → ∃ n, c n = x)
     : Function.Surjective (extractor.of allMem) := fun res =>
-  have ⟨w, p⟩ := memAll _ $ res.getFin2_mem
-  ⟨w, Fin2.getFin2_Nodup_Injective nodup $ (extractor_agrees.of _).symm.trans p⟩
+  have ⟨w, p⟩ := memAll _ $ List.get_mem _ res.val res.prop
+  ⟨w, List.nodup_iff_injective_get.mp nodup $ (extractor_agrees.of _).symm.trans p⟩
 
 noncomputable def ofFinite' (f : Finite' c) : Finite c where
   ls := f.ls
@@ -70,14 +71,15 @@ noncomputable def ofFinite' (f : Finite' c) : Finite c where
   sur := sur.of f.nodup f.memAll
 
 def memAll (fin : Finite c) (x : α) (hmem : x ∈ fin.ls) : ∃ n, c n = x := by
-  obtain ⟨w, rfl⟩ := Fin2.ofMem hmem
+  obtain ⟨w, rfl⟩ := List.get_of_mem hmem
   have ⟨w, h⟩ := fin.sur w
   obtain rfl := h.symm
   exact ⟨w, fin.extractor_agrees w⟩
 
 def allMem (fin : Finite c) (n : Nat) : c n ∈ fin.ls := by
   rw [fin.extractor_agrees n]
-  exact Fin2.getFin2_mem (fin.extractor n)
+  let this := (fin.extractor n)
+  exact List.get_mem _ this.val this.prop
 
 end equiv
 
@@ -88,16 +90,35 @@ def not_empty
 
 end C.Finite
 
-instance [PartialOrder α] {c : C α} [hc : Chain c] : Subsingleton (C.Finite c) where
+instance [PartialOrder α] {c : C α} : Subsingleton (C.Finite c) where
   allEq a b := by
+    have an := a.nodup
+    have bn := b.nodup
     rcases a with ⟨al, oa, fa, ma, sa⟩
     rcases b with ⟨bl, ob, fb, mb, sb⟩
-    have : ∀ n, al.getFin2 (fa n) = bl.getFin2 (fb n) := fun n =>
-      (ma n).symm.trans (mb n)
-    have : al = bl :=
-      sorry
-    stop
-    rfl
+    dsimp at an bn
+    obtain rfl : al = bl := by
+      apply List.eq_of_perm_of_sorted ?_ oa ob
+      apply (List.perm_ext_iff_of_nodup an bn).mpr fun el => ?_
+      rw [List.mem_iff_get, List.mem_iff_get]
+      constructor
+      <;> rintro ⟨w, h⟩
+      · obtain ⟨w, rfl⟩ := sa w
+        specialize ma w
+        obtain rfl := ma.trans h
+        exists fb w
+        exact (mb w).symm
+      · obtain ⟨w, rfl⟩ := sb w
+        specialize mb w
+        obtain rfl := mb.trans h
+        exists fa w
+        exact (ma w).symm
+    rw [C.Finite.mk.injEq]
+    refine ⟨ rfl,
+      (heq_eq_eq _ _).mpr
+      $ funext
+        (List.nodup_iff_injective_get.mp an
+        $ (ma _).symm.trans $ mb ·)⟩
 
 namespace Lub
 
@@ -142,8 +163,12 @@ class FiniteDom (α : Type _) [PartialOrder α] where
 instance [PartialOrder α] : CoeFun (FiniteDom α) (fun _ => (c : C α) → Chain c → c.Finite) where
   coe x := x.chain_fin
 
-instance [PartialOrder α] [fd : FiniteDom α] [OrderBot α] : Dom α where
+instance (priority := 500) {α} [PartialOrder α] [fd : FiniteDom α] [OrderBot α]  : Dom α where
   complete_lub c hc := Lub.finite $ fd c hc
+
+def FiniteDom.complete_eq_chain_fin {α} [Dom α] {c : C α} {hc : Chain c} [fd : FiniteDom α]
+    : complete c hc = (fd.chain_fin c hc).ls.getLast (C.Finite.not_empty _) :=
+  Lub.allEq (complete_lub c hc) (Lub.finite $ fd c hc)
 
 variable [ida : Dom α] {c : C α} {hc : Chain c}
 
@@ -154,46 +179,168 @@ def FiniteDom.complete_last
     = (fd.chain_fin c hc).ls.getLast (List.ne_nil_of_mem $ (fd.chain_fin c hc).allMem 0) :=
   Lub.allEq (complete_lub c hc) (Lub.finite (fd.chain_fin c hc))
 
-def FiniteDom.walker_lemma
-    [db : Dom β]
-    (f : α → β)
+open List in
+section
+def pw_mem
+    [DecidableRel R]
+    : {l : List α}
+    → (a ∈ pwFilter R l)
+    →  a ∈ l
+  | [], h => h
+  | x :: l, h' => by
+    if h : ∀ y ∈ pwFilter R l, R x y then
+      rw [pwFilter_cons_of_pos h, mem_cons] at h'
+      rcases h' with rfl|h'
+      · exact mem_cons_self a l
+      · exact mem_cons_of_mem x $ pw_mem h'
+    else
+      rw [pwFilter_cons_of_neg h] at h'
+      exact mem_cons_of_mem x $ pw_mem h'
+
+def pw_lift
+    [DecidableRel R]
+    : {ls : List α}
+    → List.Pairwise R' ls
+    → Pairwise R' (pwFilter R ls)
+  | [], .nil => .nil
+  | x :: l, .cons hx hl =>
+    if h : ∀ y ∈ pwFilter R l, R x y then
+      pwFilter_cons_of_pos h ▸ .cons (hx · ∘ pw_mem) (pw_lift hl)
+    else
+      pwFilter_cons_of_neg h ▸ pw_lift hl
+
+def pw_not_empty
+    [DecidableRel R]
+    : {ls : List α}
+    → ls.pwFilter R ≠ []
+    → ls ≠ []
+  | [], h => False.elim $ h rfl
+  | _ :: _, _ => List.noConfusion
+
+def not_empty_pw
+    [DecidableRel R]
+    : {ls : List α}
+    → ls ≠ []
+    → ls.pwFilter R ≠ []
+  | [], h => False.elim $ h rfl
+  | [x], _ => List.noConfusion
+  | x :: b :: l, _ =>
+    if h : ∀ y ∈ pwFilter R (b :: l), R x y then
+      pwFilter_cons_of_pos h ▸ List.noConfusion
+    else
+      pwFilter_cons_of_neg h ▸ not_empty_pw List.noConfusion
+
+def pw_filter_last
+    [DecidableRel R]
+    : {ls : List α}
+    → {nempty : ls.pwFilter R ≠ []}
+    → (ls.pwFilter R).getLast nempty = ls.getLast (pw_not_empty nempty)
+  | [], hne | [v], hne => rfl
+  | x :: hb :: tl, hne => by
+    if h : ∀ y ∈ pwFilter R (hb :: tl), R x y then
+      have h := pwFilter_cons_of_pos h
+      trans (x :: pwFilter R (hb :: tl)).getLast (h ▸ hne); congr
+      rw [List.getLast_cons (not_empty_pw List.noConfusion)]
+      exact pw_filter_last
+    else
+      have h := pwFilter_cons_of_neg h
+      trans (pwFilter R (hb :: tl)).getLast (h ▸ hne); congr
+      exact pw_filter_last
+end
+
+def sorted_of_nd_sorted
+    {α} [PartialOrder α]
+    : {ls : List α}
+    → ls.Pairwise (· ≠ ·)
+    → ls.Pairwise (· ≤ ·)
+    → ls.Pairwise (· < ·)
+  | [], .nil, .nil => .nil
+  | _ :: _, .cons hne tne, .cons hle tle =>
+    .cons (fun _ hmem => lt_of_le_of_ne (hle _ hmem) (hne _ hmem))
+      $ sorted_of_nd_sorted tne tle
+
+def nodup_mono_sorted
+    [Preorder α] [PartialOrder β] [DecidableEq β]
+    {f : α → β} (hMono : Monotone f)
+    {la : List α}
+    (hsort : List.Pairwise LT.lt la)
+    : List.Sorted LT.lt (la.map f).dedup :=
+  have sl : (List.map f la).Sorted (· ≤ ·) := by
+    induction hsort
+    · exact .nil
+    case cons h _ ih =>
+      refine .cons ?_ ih
+      intro x hmem
+      obtain ⟨x, h', rfl⟩ := List.mem_map.mp hmem
+      apply hMono $ le_of_lt (h _ h')
+  have sl := pw_lift (R := (· ≠ ·)) sl
+  have nd := List.nodup_dedup $ la.map f
+  sorted_of_nd_sorted nd sl
+
+def FiniteDom.ls_map
+    {α β}
+    [PartialOrder α]
+    [PartialOrder β]
+    [DecidableEq β]
+    [fda : FiniteDom α]
+    [fdb : FiniteDom β]
     (c : C α) (hc : Chain c)
-    : (la : List α)
-    → (lb : List β)
-    → List.Pairwise LT.lt la
-    → List.Pairwise LT.lt lb
-    → (∀ (n : ℕ), c n ∈ la)
-    → (∀ (n : ℕ), c.map f n ∈ lb)
-    → (∀ x ∈ la, ∃ n, c n = x)
-    → (∀ x ∈ lb, ∃ n, c.map f n = x)
-    → lb = List.map f la :=
-  sorry
+    (f : α → β)
+    (hMono : Monotone f)
+    : (fdb.chain_fin (c.map f) (hc.map hMono)).ls
+    = ((fda.chain_fin c hc).ls.map f).dedup := by
+  generalize chain_fin (c.map f) _ = fdb, chain_fin c hc = fda
+  have an := fda.nodup
+  have bn := fdb.nodup
+  rcases fda with ⟨la, oa, fa, ma, sa⟩
+  rcases fdb with ⟨lb, ob, fb, mb, sb⟩
+  dsimp at *
+  apply List.eq_of_perm_of_sorted ?perm ob (nodup_mono_sorted hMono oa)
+  case perm =>
+    apply (List.perm_ext_iff_of_nodup bn (List.nodup_dedup _)).mpr fun el => ?_
+    rw [List.mem_dedup, List.mem_iff_get, List.mem_iff_get]
 
-/- def FiniteDom.ls_map -/
-/-     [db : Dom β] -/
-/-     [fda : FiniteDom α] -/
-/-     [fdb : FiniteDom β] -/
-/-     (c : C α) (hc : Chain c) -/
-/-     (f : α → β) -/
-/-     (hMono : Monotone f) -/
-/-     : (fdb.chain_fin (c.map f) (hc.map hMono)).ls -/
-/-     = (fda.chain_fin c hc).ls.map f := by -/
-/-   have fda := chain_fin c hc -/
-/-   have fdb := chain_fin (c.map f) (hc.map hMono) -/
-/-   rcases fda with ⟨la, oa, ama, maa⟩ -/
-/-   rcases fdb with ⟨lb, ob, amb, mab⟩ -/
-/-   apply walker_lemma f c hc la lb -/
-
-
+    have p₁ := (List.length_map la f)
+    constructor
+    <;> rintro ⟨w, h⟩
+    · obtain ⟨w, rfl⟩ := sb w
+      specialize mb w
+      obtain rfl := mb.trans h
+      exists cast (congr rfl p₁.symm) (fa w)
+      rw [List.get_map]
+      congr
+      rw [←(ma w).symm]
+      congr
+      exact cast_heq (congr rfl p₁.symm) (fa w)
+    · obtain ⟨w', p⟩ := sa (cast (congr rfl p₁) w)
+      specialize ma w'
+      subst h
+      rw [List.get_map]
+      exists fb w'
+      exact (mb w').symm.trans
+        $ congr (rfl (a := f))
+        $ ma.trans
+        $ congr rfl
+        $ p.trans
+        $ cast_eq_iff_heq.mpr
+        $ (Fin.heq_ext_iff p₁).mpr rfl
 end
 
 section
 
 variable [Dom D] [Dom E]
 
-def Continous.finite [dd : FiniteDom D] [de : FiniteDom E] {f : D → E} (fmono : Monotone f) : Continous.Helper f where
+def Continous.finite [DecidableEq E] [dd : FiniteDom D] [de : FiniteDom E] {f : D → E} (fmono : Monotone f) : Continous f where
   mono := fmono
-  preserves_lubs c hc := sorry
+  preserves_lubs c hc := by
+    repeat rw [FiniteDom.complete_eq_chain_fin]
+    have eq' := FiniteDom.ls_map c hc f fmono
+    have pnempty := C.Finite.not_empty (FiniteDom.chain_fin (c.map f) (Chain.map fmono))
+    have pne' : ((FiniteDom.chain_fin c hc).ls.map f).dedup ≠ [] :=
+      not_empty_pw $ fun x =>
+        C.Finite.not_empty (FiniteDom.chain_fin c hc) $ List.map_eq_nil.mp x
+    have : (FiniteDom.chain_fin (c.map f) (Chain.map fmono)).ls.getLast pnempty = ((FiniteDom.chain_fin c hc).ls.map f).dedup.getLast pne' := by congr
+    simp only [this, List.dedup, pw_filter_last, List.getLast_map]
 
 end
 
