LeanScratch/HEq.lean
@@ -1,0 +1,25 @@
+@[elab_as_elim]
+def HEq.dependentRw
+    {α : Sort _} {a b : α}
+    {submotive : α → Sort _} {motive : (base : α) → submotive base → Sort _}
+    {x : submotive a} {y : submotive b}
+    (hParEq : a = b)
+    (hEq : HEq x y)
+    (src : motive a x)
+    : motive b y := by
+  subst hParEq
+  subst hEq
+  exact src
+
+@[elab_as_elim]
+def HEq.dependentRw'
+    {α : Sort _} {a b : α}
+    {submotive : α → Sort _} {motive : (base : α) → submotive base → Sort _}
+    {x : submotive a} {y : submotive b}
+    (hParEq : a = b)
+    (hEq : HEq x y)
+    (src : motive a x)
+    : motive b y := by
+  subst hParEq
+  subst hEq
+  exact src
